In-class graphs.v

graphs.v
@@ -22,6 +22,17 @@ Proof.
   apply Pos.eqb_refl.
 Qed.  
 
+Lemma node_eqbP :
+  forall x y : node,
+    reflect (x = y) (node_eqb x y).
+Proof.
+  intros.
+  destruct (node_eqb x y) eqn:H.
+  rewrite node_eqb_eq in H. constructor; auto.
+  constructor; intros H2; rewrite H2, node_eqb_refl in H.
+  congruence.
+Qed.  
+
 (** Undirected Graphs *)
 
 Inductive graph : Type :=
@@ -39,12 +50,52 @@ Example ex1 : graph :=
        (Node 2 (3 :: nil)
              (Node 3 nil Empty)).
 
-Fixpoint neighbors_of (x : node) (g : graph) : list node :=
+Example ex2 : graph :=
+  Node 3 (2 :: 1 :: nil)
+       (Node 2 (1 :: nil)
+             (Node 1 nil Empty)).
+
+(** Return the adjacency list associated by graph g
+    with node x. *)
+
+Fixpoint adj_of (x : node) (g : graph) : list node :=
   match g with
   | Empty => nil
   | Node y adj g' =>
     if node_eqb x y then adj
-    else neighbors_of x g'
+    else adj_of x g'
+  end.
+
+(** Return all neighbors in g of node x. *)
+
+Fixpoint nodelist_contains (x : node) (l : list node) : bool :=
+  match l with
+  | nil => false
+  | y :: l' =>
+    if node_eqb x y then true
+    else nodelist_contains x l'
+    (* node_eqb x y || nodelist_contains x l' *)
+  end.
+
+Lemma nodelist_containsP :
+  forall x l,
+    reflect (In x l) (nodelist_contains x l).
+Proof.
+  induction l; try constructor; auto.
+  simpl. destruct (node_eqbP x a).
+  constructor; auto.
+  destruct (nodelist_contains x l) eqn:H.
+  constructor. right. inversion IHl; auto.
+  constructor. intros [H2|H2]. subst x. auto. inversion IHl; auto.
+Qed.  
+
+Fixpoint neighbors_of (x : node) (g : graph) : list node :=
+  match g with
+  | Empty => nil
+  | Node y adj g' =>
+    if node_eqb x y then adj ++ neighbors_of x g'
+    else if nodelist_contains x adj then y :: neighbors_of x g'
+         else neighbors_of x g'
   end.
 
 Fixpoint graph_contains (x : node) (g : graph) : bool :=
@@ -91,8 +142,40 @@ Proof.
   apply H.
 Qed.    
 
+Lemma ex1_graph_ok : graph_ok ex1.
+Proof.
+  unfold ex1; repeat (constructor; auto).
+  (*apply NodeOk; auto.
+  apply NodeOk; auto.
+  apply NodeOk; auto.
+  apply EmptyOk.*)
+Qed.  
+
+Lemma filter_property :
+  forall (A : Type) (l : list A) (f : A -> bool),
+    forallb f (filter f l) = true.
+Proof.
+  induction l.
+  { simpl. auto. }
+  simpl. intros f. destruct (f a) eqn:H.
+  { simpl. rewrite H. simpl. apply IHl. }
+  apply IHl.
+Qed.  
+
 Definition remove (x : node) (adj : list node) : list node :=
   filter (fun z => negb (node_eqb x z)) adj.
+
+Lemma remove_app :
+  forall x l1 l2,
+    remove x (l1 ++ l2) = remove x l1 ++ remove x l2.
+Proof.
+  unfold remove.
+  intros x l1 l2.
+  induction l1; auto.
+  simpl.
+  destruct (negb _); auto.
+  simpl. f_equal. auto.
+Qed.  
 
 Lemma In_remove_weaken :
   forall x y l,
@@ -119,6 +202,22 @@ Proof.
   auto.
 Qed.    
 
+Lemma not_In_remove_eq :
+  forall x y l,
+    In y l -> ~In y (remove x l) -> x = y.
+Proof.
+  intros x y.
+  induction l; auto.
+  { simpl. congruence. }
+  simpl. intros [H|H].
+  { subst y. intros H.
+    destruct (negb _) eqn:H2.
+    rewrite not_in_cons in H. destruct H. exfalso; apply H; auto.
+    destruct (node_eqbP x a); auto. simpl in H2. congruence. }
+  destruct (node_eqbP x a); auto.
+  unfold negb. rewrite not_in_cons. intros [H1 H2]. auto.
+Qed.  
+
 Fixpoint remove_node (x : node) (g : graph) : graph :=
   match g with
   | Empty => Empty
@@ -139,10 +238,22 @@ Proof.
     destruct (node_eqb y x) eqn:H3.
     { rewrite node_eqb_eq in H3; subst y.
       exfalso; apply H; auto. }
-    auto. }
+    rewrite IHg.
+    destruct (nodelist_contains _ _); auto.
+    simpl. rewrite node_eqb_refl. auto. }
   destruct (node_eqb y n) eqn:H3.
-  { simpl; rewrite H3; auto. }
-  simpl. rewrite H3. apply IHg.
+  { simpl; rewrite H3; auto.
+    rewrite IHg, remove_app; auto. }
+  simpl. rewrite H3.
+  destruct (nodelist_containsP y (remove x l)).
+  { destruct (nodelist_containsP y l).
+    simpl. rewrite H2. simpl. rewrite IHg. auto.
+    destruct (nodelist_containsP y l). congruence.
+    destruct (nodelist_containsP y (remove x l)); [|congruence].
+    apply In_remove_weaken in i; contradiction. }
+  destruct (nodelist_containsP y l); auto.
+  simpl. rewrite H2. simpl. rewrite IHg.
+  exfalso. apply H. apply not_In_remove_eq in n0; auto.
 Qed.    
 
 Lemma remove_node_contains :
@@ -193,4 +304,21 @@ Proof.
   inversion H; subst.
   auto.
 Qed.      
-    
+
+(** Other potential operators/predicates/definitions: 
+    - definition of paths from x <-> y
+    - does such a path exist between x <-> y? 
+    - graph union 
+    - set of vertices 
+    - set of edges 
+    - induced graph for a given set of vertices 
+    - graph isomorphism (predicate over a labeling from 
+      one graph to the other)
+    - definitions of independent sets, maximal independent sets, etc. 
+
+    Other possible projects: 
+    - Is there a graph invariant that implies: 
+      "graph isomorphism implies syntactic equality"?
+    - Abstract interface over "inductive graphs", together with 
+      associated induction principle, plus faster implementation
+ *)
